#196 everything finished (some sorrys left)

automat/ndaComplete.thy
@@ -21,9 +21,9 @@ imports ndAutomaton
 begin
 
 type_synonym ('state, 'm) nda2TransF = "('state, 'm) ndAutomaton \<Rightarrow>
-    (('state \<times> 'm sbElem) \<Rightarrow> (('state \<times> 'm SB) set rev))"
+    (('state \<times> 'm sbElem) \<Rightarrow> (('state \<times> 'm SB) set))"
 
-type_synonym ('state, 'm) nda2InitStateF = "('state, 'm) ndAutomaton \<Rightarrow> (('state \<times> 'm SB) set rev)"
+type_synonym ('state, 'm) nda2InitStateF = "('state, 'm) ndAutomaton \<Rightarrow> (('state \<times> 'm SB) set)"
 
 (*******************************************************************)
 section \<open>Definition\<close>
@@ -31,30 +31,30 @@ section \<open>Definition\<close>
 
 subsection \<open>predicate\<close>
 
-definition transIsComplete:: "(('state \<times> 'm::message sbElem) \<Rightarrow> (('state \<times> 'm SB) set rev)) \<Rightarrow>
+definition transIsComplete:: "(('state \<times> 'm::message sbElem) \<Rightarrow> (('state \<times> 'm SB) set)) \<Rightarrow>
   bool" where 
-"transIsComplete \<equiv> \<lambda> trans. \<forall> state sbe. trans (state, sbe) \<noteq> Rev {}"
+"transIsComplete \<equiv> \<lambda> trans. \<forall> state sbe. trans (state, sbe) \<noteq> {}"
 
 definition ndaIsComplete:: "('state::type, 'm::message) ndAutomaton \<Rightarrow> bool" where
-"ndaIsComplete \<equiv> \<lambda> nda. transIsComplete (ndaTransition\<cdot>nda) \<and> ndaInitialState\<cdot>nda \<noteq> Rev {}"   
+"ndaIsComplete \<equiv> \<lambda> nda. transIsComplete (ndaTransition\<cdot>nda) \<and> ndaInitialState\<cdot>nda \<noteq> {}"   
 
 
 subsection \<open>transCompletion\<close>
 
 (* Ignore completion: stay in the same state and produce empty SB *)
 definition ignoreTrans_h:: "('state::type \<times> 'm::message sbElem) \<Rightarrow>
-    ('state \<times> 'm SB) set rev" where
-"ignoreTrans_h \<equiv> \<lambda> (state, sbe). Rev {(state, ubLeast UNIV)}"
+    ('state \<times> 'm SB) set" where
+"ignoreTrans_h \<equiv> \<lambda> (state, sbe). {(state, ubLeast UNIV)}"
 
 (* Chaos completion: switch to an abitrary state and produce abitrary output *)
 definition chaosTrans_h:: "('state::type \<times> 'm::message sbElem) \<Rightarrow>
-    ('state \<times> 'm SB) set rev" where
-"chaosTrans_h \<equiv>  \<lambda> (state, sbe). Rev UNIV"
+    ('state \<times> 'm SB) set" where
+"chaosTrans_h \<equiv>  \<lambda> (state, sbe). UNIV"
 
 (* *)
-definition transCompletion:: "(('state::type \<times> 'm::message sbElem) \<Rightarrow> ('state \<times> 'm SB) set rev) 
+definition transCompletion:: "(('state::type \<times> 'm::message sbElem) \<Rightarrow> ('state \<times> 'm SB) set) 
   \<Rightarrow> ('state, 'm::message) nda2TransF"
-  where "transCompletion f \<equiv> (\<lambda> nda. (\<lambda> (state, sbe). if ((ndaTransition\<cdot>nda) (state,sbe)  = Rev {}) then 
+  where "transCompletion f \<equiv> (\<lambda> nda. (\<lambda> (state, sbe). if ((ndaTransition\<cdot>nda) (state,sbe)  = {}) then 
                 f (state, sbe) else ((ndaTransition\<cdot>nda) (state,sbe))))"
 
 (* DD: error completion - unknown transition will cause the automaton to switch to error state and
@@ -62,10 +62,10 @@ and it will stay there and produce no output (empty SB). To ensure that it will 
 it will stay in the error state for ever (see Steffen's MD)  *)
 definition errorTransCompletion:: "'state::type \<Rightarrow> ('state, 'm::message) nda2TransF"
   where "errorTransCompletion errorState nda \<equiv> 
-let errorStateP = (\<lambda> trans (state, sbe). trans (state,sbe)  = Rev {} \<or>
+let errorStateP = (\<lambda> trans (state, sbe). trans (state,sbe)  = {} \<or>
                                          state = errorState)
 in (\<lambda> (state, sbe). if (errorStateP (ndaTransition\<cdot>nda) (state,sbe)) then 
-                Rev {(errorState, ubLeast UNIV)} else ((ndaTransition\<cdot>nda) (state,sbe)))"
+                {(errorState, ubLeast UNIV)} else ((ndaTransition\<cdot>nda) (state,sbe)))"
 
 abbreviation ignorerTransCompletion:: "('state, 'm::message) nda2TransF"
   where "ignorerTransCompletion \<equiv> \<lambda> trans. transCompletion ignoreTrans_h trans"
@@ -75,15 +75,15 @@ abbreviation chaosTransCompletion:: "('state, 'm::message) nda2TransF"
 
 
 subsection \<open>InitStateCompletion\<close>
-definition errorInit_h::  "'state  \<Rightarrow> (('state \<times> 'm::message SB) set rev)" where
-"errorInit_h \<equiv> \<lambda> state. Rev {(state, ubLeast UNIV)}"
+definition errorInit_h::  "'state  \<Rightarrow> (('state \<times> 'm::message SB) set)" where
+"errorInit_h \<equiv> \<lambda> state. {(state, ubLeast UNIV)}"
 
-definition chaosInit_h:: "(('state \<times> 'm SB) set rev)" where
-"chaosInit_h \<equiv> Rev UNIV"
+definition chaosInit_h:: "(('state \<times> 'm SB) set)" where
+"chaosInit_h \<equiv> UNIV"
 
-definition initCompletion:: "(('state \<times> 'm SB) set rev) \<Rightarrow> 
+definition initCompletion:: "(('state \<times> 'm SB) set) \<Rightarrow> 
    ('state::type, 'm::message) nda2InitStateF"
-  where "initCompletion \<equiv> \<lambda> otherInit nda.  if (ndaInitialState\<cdot>nda = Rev {}) then otherInit else
+  where "initCompletion \<equiv> \<lambda> otherInit nda.  if (ndaInitialState\<cdot>nda = {}) then otherInit else
                                     ndaInitialState\<cdot>nda"
 
 lift_definition ndaCompletion:: "('state::type, 'm::message) nda2TransF \<Rightarrow>
@@ -111,11 +111,11 @@ section \<open>Lemma\<close>
 (*******************************************************************)
 
 lemma ndaiscomplI: assumes "transIsComplete (ndaTransition\<cdot>nda)"
-  and "ndaInitialState\<cdot>nda \<noteq> Rev {}"
+  and "ndaInitialState\<cdot>nda \<noteq> {}"
   shows "ndaIsComplete nda"
   by (simp add: assms(1) assms(2) ndaIsComplete_def)
 
-lemma traniscomplI: assumes "\<And> state sbe. transition (state, sbe) \<noteq> Rev {}"
+lemma traniscomplI: assumes "\<And> state sbe. transition (state, sbe) \<noteq> {}"
   shows "transIsComplete transition"
   by (simp add: assms ndaIsComplete_def transIsComplete_def)
 
@@ -135,7 +135,7 @@ lemma transcompl_complI: assumes "transIsComplete f"
 lemma ndaChaosCompletion_true: "ndaIsComplete (ndaChaosCompletion nda)"
   apply (rule ndaiscomplI)
    apply (simp_all add: ndaCompletion_def ndaTransition_def)
-   apply (metis (no_types) Rep_ndAutomaton_inverse eq_fst_iff ignoreTrans_h_def insert_not_empty inv_rev_rev ndaCompletion.rep_eq old.prod.case transIsComplete_def transcompl_complI)
+   apply (metis (no_types) Rep_ndAutomaton_inverse eq_fst_iff ignoreTrans_h_def insert_not_empty ndaCompletion.rep_eq old.prod.case transIsComplete_def transcompl_complI)
   by (simp add: Abs_ndAutomaton_inverse chaosInit_h_def initCompletion_def ndaInitialState.rep_eq)
 
 lemma ndaErrorCompletion_true: "ndaIsComplete (ndaErrorCompletion state nda)"
