automat/ndAutomaton.thy
@@ -865,20 +865,20 @@ qed
 
 
 lemma nda_h_final_back_eq: assumes "\<And>state sbe. sbeDom sbe = ndaDom\<cdot>nda \<Longrightarrow> 
-spsConcIn (sbe2SB sbe) (other state) = 
+spsConcIn (sbe2SB sbe)\<cdot>(other state) = 
   ndaConcOutFlatten (ndaDom\<cdot>nda) (ndaRan\<cdot>nda) ((ndaTransition\<cdot>nda) (state,sbe)) (other)"
-  and "\<And> state sbe. (ndaTransition\<cdot>nda) (state, sbe) \<noteq> Rev {}"
-  and "\<And> state. other state \<noteq> uspecMax (ndaDom\<cdot>nda) (ndaRan\<cdot>nda)"
+  and "\<And> state sbe. (ndaTransition\<cdot>nda) (state, sbe) \<noteq> {}"
+  and "\<And> state. other state \<noteq> uspecLeast (ndaDom\<cdot>nda) (ndaRan\<cdot>nda)"
   and "\<And> state. uspecIsStrict (other state)"
   and "\<And> state. uspecDom\<cdot>(other state) = ndaDom\<cdot>nda" 
   and "\<And> state. uspecRan\<cdot>(other state) = ndaRan\<cdot>nda"
 
   and "\<And>x state sbe. uspecIsStrict (x state) \<Longrightarrow> uspecDom\<cdot>(x state) = ndaDom\<cdot>nda \<Longrightarrow> uspecRan\<cdot>(x state) = ndaRan\<cdot>nda
-    \<Longrightarrow> sbeDom sbe = ndaDom\<cdot>nda \<Longrightarrow> spsConcIn (sbe2SB sbe) (x state) =  ndaConcOutFlatten (ndaDom\<cdot>nda) (ndaRan\<cdot>nda) ((ndaTransition\<cdot>nda) (state,sbe)) (x)
-    \<Longrightarrow> other \<sqsubseteq> x"
+    \<Longrightarrow> sbeDom sbe = ndaDom\<cdot>nda \<Longrightarrow> spsConcIn (sbe2SB sbe)\<cdot>(x state) =  ndaConcOutFlatten (ndaDom\<cdot>nda) (ndaRan\<cdot>nda) ((ndaTransition\<cdot>nda) (state,sbe)) (x)
+    \<Longrightarrow> x \<sqsubseteq> other "
 shows "nda_h nda = other" 
   apply(simp add: nda_h_def)
-  apply(subst lfp_least_eq, auto simp add: assms)
+  apply(subst gfp_greatest_eq, auto simp add: assms)
   apply (simp add: nda_h_inner_monofun)
   apply (simp add: nda_inner_good)
      apply (simp add: nda_h_valid_domain)
